Generalize delimiter combinator; disabling automation for now.

src/Narcissus/BinLib/AlignedDelimiter.v
@@ -7,169 +7,143 @@ Require Import
         Fiat.Narcissus.BinLib.AlignedByteString
         Fiat.Narcissus.BinLib.AlignedEncodeMonad
         Fiat.Narcissus.BinLib.AlignedDecodeMonad
-        Fiat.Narcissus.BinLib.AlignWord
-        Fiat.Narcissus.BinLib.AlignedString.
-
-Require Import Coq.Strings.String.
+        Fiat.Narcissus.BinLib.AlignWord.
 
 Section AlignedDelimter.
-
+  Context {A : Type}.
   Context {cache : Cache}.
-  Context {cacheAddNat : CacheAdd cache nat}.
-
-  Variable addD_addD_plus :
-    forall (cd : CacheDecode) (n m : nat), addD (addD cd n) m = addD cd (n + m).
-
-  Variable addE_addE_plus :
-    forall (ce : CacheFormat) (n m : nat), addE (addE ce n) m = addE ce (n + m).
-  Variable addE_0 :
-    forall (ce : CacheFormat), addE ce 0 = ce.
-
-  Variable open : string.
-  Variable close : string.
 
   Open Scope AlignedEncodeM_scope.
 
-  Definition AlignedEncodeDelimiter {A}
+  Definition AlignedEncodeDelimiter
+             (encode_open : forall sz, AlignedEncodeM (S := unit) sz)
+             (encode_close : forall sz, AlignedEncodeM (S := unit) sz)
              (encode_A : forall sz, AlignedEncodeM (S := A) sz)
              sz
     : AlignedEncodeM (S := A) sz :=
-    (fun v idx _ => AlignedEncodeString sz v idx open) >> encode_A sz >>
-    (fun v idx _ => AlignedEncodeString sz v idx close).
+    (fun v idx _ => encode_open sz v idx tt) >> encode_A sz >>
+      (fun v idx _ => encode_close sz v idx tt).
 
-  Lemma CorrectAlignedEncoderForFormatDelimiter {A}
-        format_A
-        encode_A
-        (encode_A_OK : CorrectAlignedEncoder format_A encode_A)
-        (* These two side-conditions can be easily discharged when the cache is
-        empty. *)
-        (encode_A_OK1 :
-           forall (a : A) (env : CacheFormat) (tenv' tenv'' : ByteString * CacheFormat),
-            format_A a env ∋ tenv' ->
-            Projection_Format format_string (constant close) a (snd tenv') ∋ tenv'' ->
-            exists tenv3 tenv4 : _ * CacheFormat,
-              projT1 encode_A_OK a env = Some tenv3
-              /\ Projection_Format format_string (constant close) a (snd tenv3) ∋ tenv4)
-        (encode_A_OK2 :
-           forall (a : A) (env : CacheFormat) (tenv' tenv'' : ByteString * CacheFormat),
-             (format_string ◦ constant open) a env ∋ tenv' ->
-             format_with_term format_A close a (snd tenv') ∋ tenv'' ->
-            exists tenv3 tenv4 : _ * CacheFormat,
-              projT1 (CorrectAlignedEncoderForProjection_Format
-                        (constant open) format_string
-                        AlignedEncodeString
-                        (CorrectAlignedEncoderForFormatString addE_addE_plus addE_0))
-                     a env = Some tenv3
-              /\ format_with_term format_A close a (snd tenv3) ∋ tenv4)
-    : CorrectAlignedEncoder (format_delimiter (A:=A) open close format_A)
-                            (AlignedEncodeDelimiter encode_A).
+
+  Lemma CorrectAlignedEncoderForFormatDelimiter
+    format_open encode_open
+    format_close encode_close
+    format_A encode_A
+    (encode_open_OK : CorrectAlignedEncoder format_open encode_open)
+    (encode_close_OK : CorrectAlignedEncoder format_close encode_close)
+    (encode_A_OK : CorrectAlignedEncoder format_A encode_A)
+    (* The following two conditions can be easily discharged when cache is
+    empty. *)
+    (encode_A_OK1 :
+      forall s env tenv' tenv'',
+        format_A s env ∋ tenv' ->
+        (format_close ◦ constant tt) s (snd tenv') ∋ tenv'' ->
+        exists tenv3 tenv4,
+          projT1 encode_A_OK s env = Some tenv3 /\
+            (format_close ◦ constant tt) s (snd tenv3) ∋ tenv4)
+    (encode_A_OK2 :
+      forall s env tenv' tenv'',
+        (format_open ◦ constant tt) s env ∋ tenv' ->
+        format_with_term format_close format_A s (snd tenv') ∋ tenv'' ->
+        exists tenv3 tenv4,
+          projT1
+            (CorrectAlignedEncoderForProjection_Format (constant ()) format_open
+               encode_open encode_open_OK) s env = Some tenv3 /\
+            format_with_term format_close format_A s (snd tenv3) ∋ tenv4)
+    : CorrectAlignedEncoder (S:=A)
+        (format_delimiter format_open format_close format_A)
+        (AlignedEncodeDelimiter encode_open encode_close encode_A).
   Proof.
-    repeat (eapply CorrectAlignedEncoderForThenC; [| unshelve instantiate (1:=_)]; eauto);
-    eapply CorrectAlignedEncoderForProjection_Format; eapply CorrectAlignedEncoderForFormatString; eauto.
+    repeat (eapply CorrectAlignedEncoderForThenC;
+            [| unshelve instantiate (1:=_)]; eauto);
+    eapply CorrectAlignedEncoderForProjection_Format; eauto.
   Qed.
 
   Open Scope AlignedDecodeM_scope.
 
-  Definition AlignedDecodeDelimiter {A}
-             (decode_A_with_term : string -> forall {m}, AlignedDecodeM A m)
-             {m}
-    : AlignedDecodeM A m :=
-    s <- AlignedDecodeString (length open);
-    if String.eqb open s
-    then decode_A_with_term close
-    else ThrowAlignedDecodeM.
+  Variable decode_open : DecodeM (unit * ByteString) ByteString.
+  Variable decode_close : DecodeM (unit * ByteString) ByteString.
+  Variable decode_A : DecodeM (A * ByteString) ByteString.
+  Variable decode_open_aligned : forall {m}, AlignedDecodeM unit m.
+  Variable decode_close_aligned : forall {m}, AlignedDecodeM unit m.
+  Variable decode_A_aligned : forall {m}, AlignedDecodeM A m.
+  Variable decode_open_OK :
+      DecodeMEquivAlignedDecodeM decode_open (@decode_open_aligned).
+  Variable decode_close_OK :
+      DecodeMEquivAlignedDecodeM decode_close (@decode_close_aligned).
+  Variable decode_A_OK :
+      DecodeMEquivAlignedDecodeM decode_A (@decode_A_aligned).
 
-  Lemma AlignedDecodeDelimiterM {A C : Type}
-        (decode_A_with_term : string -> DecodeM (A * _) ByteString)
-        (decode_A_with_term_aligned : string -> forall {m}, AlignedDecodeM A m)
+  Definition AlignedDecodeDelimiter
+    (decode_with_term_aligned : forall {m}, AlignedDecodeM A m)
+    {m}
+    : AlignedDecodeM A m :=
+    _ <- decode_open_aligned; decode_with_term_aligned.
+
+  Lemma AlignedDecodeDelimiterM {C : Type}
+        (decode_with_term : DecodeM (A * _) ByteString)
+        (decode_with_term_aligned : forall {m}, AlignedDecodeM A m)
     : forall (t : A -> DecodeM (C * _) ByteString)
-             (t' : A -> forall {numBytes}, AlignedDecodeM C numBytes),
-      (forall s, DecodeMEquivAlignedDecodeM (decode_A_with_term s)
-                                       (@decode_A_with_term_aligned s)) ->
+        (t' : A -> forall {numBytes}, AlignedDecodeM C numBytes),
+      DecodeMEquivAlignedDecodeM decode_with_term (@decode_with_term_aligned) ->
       (forall b, DecodeMEquivAlignedDecodeM (t b) (@t' b))
       -> DecodeMEquivAlignedDecodeM
-           (fun v cd => `(a, bs, cd') <- decode_delimiter open close decode_A_with_term
-                                                        v cd;
+           (fun v cd => `(a, bs, cd') <- decode_delimiter decode_open
+                                         decode_with_term v cd;
                           t a bs cd')
-           (fun numBytes => a <- AlignedDecodeDelimiter decode_A_with_term_aligned;
+           (fun numBytes => a <- AlignedDecodeDelimiter
+                                 (@decode_with_term_aligned);
                             t' a).
   Proof.
     intros.
     eapply Bind_DecodeMEquivAlignedDecodeM; eauto.
     eapply Bind_DecodeMEquivAlignedDecodeM; eauto.
-    eapply AlignedDecodeStringM'.
-    intros. eapply AlignedDecode_ifb; eauto.
   Qed.
 
-  Definition AlignedDecodeWithTermStringSimple {A}
-             (decode_A : forall {m}, AlignedDecodeM A m)
-             (close : string)
-             {m}
+  Definition AlignedDecodeWithTermSimple {m}
     : AlignedDecodeM A m :=
-    a <- decode_A;
-    s <- AlignedDecodeString (length close);
-    if String.eqb close s
-    then return a
-    else ThrowAlignedDecodeM.
+    a <- decode_A_aligned; _ <- decode_close_aligned; return a.
 
-  Theorem AlignedDecodeWithTermStringSimpleM' {A : Type}
-        (decode_A : DecodeM (A * _) ByteString)
-        (decode_A_aligned : forall {m}, AlignedDecodeM A m)
-    : DecodeMEquivAlignedDecodeM decode_A (@decode_A_aligned) ->
-      forall close,
-        DecodeMEquivAlignedDecodeM
-          (decode_with_term_simple decode_A close)
-          (fun numBytes => AlignedDecodeWithTermStringSimple
-                           (@decode_A_aligned) close).
+  Theorem AlignedDecodeWithTermSimpleM'
+    : DecodeMEquivAlignedDecodeM
+        (decode_with_term_simple decode_close decode_A)
+        (fun numBytes => AlignedDecodeWithTermSimple).
   Proof.
-    intros.
-    eapply Bind_DecodeMEquivAlignedDecodeM; eauto.
-    intros. eapply AlignedDecodeStringM.
-    intros. eapply AlignedDecode_ifb.
-    eapply Return_DecodeMEquivAlignedDecodeM.
+    intros; eapply Bind_DecodeMEquivAlignedDecodeM; eauto.
+    intros; eapply Bind_DecodeMEquivAlignedDecodeM; eauto.
+    intros. eapply Return_DecodeMEquivAlignedDecodeM.
   Qed.
 
-  Theorem AlignedDecodeWithTermStringSimpleM {A C : Type}
-        (decode_A : DecodeM (A * _) ByteString)
-        (decode_A_aligned : forall {m}, AlignedDecodeM A m)
+  Theorem AlignedDecodeWithTermSimpleM {C : Type}
     : forall (t : A -> DecodeM (C * _) ByteString)
-             (t' : A -> forall {numBytes}, AlignedDecodeM C numBytes),
-      DecodeMEquivAlignedDecodeM decode_A (@decode_A_aligned) ->
+        (t' : A -> forall {numBytes}, AlignedDecodeM C numBytes),
       (forall b, DecodeMEquivAlignedDecodeM (t b) (@t' b)) ->
-      forall close,
-        DecodeMEquivAlignedDecodeM
-           (fun v cd => `(a, bs, cd') <- decode_with_term_simple
-                                         decode_A close v cd;
-                          t a bs cd')
-           (fun numBytes => a <- AlignedDecodeWithTermStringSimple
-                                 (@decode_A_aligned) close;
-                            t' a).
+      DecodeMEquivAlignedDecodeM
+        (fun v cd => `(a, bs, cd') <- decode_with_term_simple
+                                      decode_close decode_A v cd;
+                       t a bs cd')
+        (fun numBytes => a <- AlignedDecodeWithTermSimple;
+                         t' a).
   Proof.
-    eauto using Bind_DecodeMEquivAlignedDecodeM, AlignedDecodeWithTermStringSimpleM'.
+    eauto using Bind_DecodeMEquivAlignedDecodeM, AlignedDecodeWithTermSimpleM'.
   Qed.
 
-  Definition AlignedDecodeDelimiterSimple {A}
-             (decode_A : forall {m}, AlignedDecodeM A m)
-             {m}
+  Definition AlignedDecodeDelimiterSimple {m}
     : AlignedDecodeM A m :=
-    AlignedDecodeDelimiter (AlignedDecodeWithTermStringSimple (@decode_A)).
+    AlignedDecodeDelimiter (@AlignedDecodeWithTermSimple).
 
-  Theorem AlignedDecodeDelimiterSimpleM {A C : Type}
-        (decode_A : DecodeM (A * _) ByteString)
-        (decode_A_aligned : forall {m}, AlignedDecodeM A m)
+  Theorem AlignedDecodeDelimiterSimpleM {C : Type}
     : forall (t : A -> DecodeM (C * _) ByteString)
-             (t' : A -> forall {numBytes}, AlignedDecodeM C numBytes),
-      DecodeMEquivAlignedDecodeM decode_A (@decode_A_aligned) ->
+        (t' : A -> forall {numBytes}, AlignedDecodeM C numBytes),
       (forall b, DecodeMEquivAlignedDecodeM (t b) (@t' b))
       -> DecodeMEquivAlignedDecodeM
            (fun v cd => `(a, bs, cd') <- decode_delimiter_simple
-                                         open close decode_A v cd;
+                                         decode_open decode_close decode_A v cd;
                           t a bs cd')
-           (fun numBytes => a <- AlignedDecodeDelimiterSimple
-                                 (@decode_A_aligned);
+           (fun numBytes => a <- AlignedDecodeDelimiterSimple;
                             t' a).
   Proof.
-    eauto using AlignedDecodeDelimiterM, AlignedDecodeWithTermStringSimpleM'.
+    eauto using AlignedDecodeDelimiterM, AlignedDecodeWithTermSimpleM'.
   Qed.
 
 End AlignedDelimter.
