src/Narcissus/BinLib/WithTerm/String.v
@@ -15,30 +15,26 @@ Section String.
   Context {cache : Cache}.
   Context {cacheAddNat : CacheAdd cache nat}.
 
-  Variable addD_addD_plus :
-    forall (cd : CacheDecode) (n m : nat), addD (addD cd n) m = addD cd (n + m).
-
-  Variable addE_addE_plus :
-    forall (ce : CacheFormat) (n m : nat), addE (addE ce n) m = addE ce (n + m).
-  Variable addE_0 :
-    forall (ce : CacheFormat), addE ce 0 = ce.
+  Variable decode_close_aligned : forall {m}, AlignedDecodeM unit m.
 
   Open Scope AlignedDecodeM_scope.
 
   Definition AlignedDecodeStringWithTerm {m}
-             (close : string)
     : AlignedDecodeM string m.
   Admitted.
 
+  Variable decode_close : DecodeM (unit * ByteString) ByteString.
+  Variable decode_close_OK :
+      DecodeMEquivAlignedDecodeM decode_close (@decode_close_aligned).
+
   Lemma AlignedDecodeStringWithTermM {C : Type}
-        (close : string)
     : forall (t : string -> DecodeM (C * _) ByteString)
-             (t' : string -> forall {numBytes}, AlignedDecodeM C numBytes),
+        (t' : string -> forall {numBytes}, AlignedDecodeM C numBytes),
       (forall b, DecodeMEquivAlignedDecodeM (t b) (@t' b))
       -> DecodeMEquivAlignedDecodeM
-           (fun v cd => `(s, bs, cd') <- decode_string_with_term close v cd;
+           (fun v cd => `(s, bs, cd') <- decode_string_with_term decode_close v cd;
                       t s bs cd')
-           (fun numBytes => s <- AlignedDecodeStringWithTerm close;
+           (fun numBytes => s <- AlignedDecodeStringWithTerm;
                           t' s).
   Proof.
   Admitted.
