src/Narcissus/Formats/Delimiter.v
@@ -4,170 +4,133 @@ Require Import
         Fiat.Narcissus.Common.EquivFormat
         Fiat.Narcissus.Formats.Base.FMapFormat
         Fiat.Narcissus.Formats.Base.SequenceFormat
-        Fiat.Narcissus.Formats.StringOpt
         Fiat.Narcissus.Formats.Empty
         Fiat.Narcissus.Formats.Sequence.
-Require Import
-        Coq.Strings.String.
 
 Section Delimiter.
   Context {A : Type}.
   Context {T : Type}.
   Context {cache : Cache}.
-  Context {cacheAddNat : CacheAdd cache nat}.
   Context {monoid : Monoid T}.
   Context {monoidUnit : QueueMonoidOpt monoid bool}.
 
-  (* [open] and [close] will probably be formats in the future to support XML
-  tag with attributes and whitespaces. *)
-  Variable open : string.
-  Variable close : string.
+  Variable format_open : FormatM unit T.
+  Variable decode_open : DecodeM (unit * T) T.
+
+  Variable format_close : FormatM unit T.
+  Variable decode_close : DecodeM (unit * T) T.
 
   Variable format_A : FormatM A T.
+  Variable decode_A : DecodeM (A * T) T.
+  Variable A_predicate : A -> Prop.
   Variable A_cache_inv : CacheDecode -> Prop.
-  Variable A_cache_OK : cache_inv_Property A_cache_inv
-                                           (fun P => forall b cd, P cd -> P (addD cd b)).
 
-  Definition format_with_term (close : string) : FormatM A T :=
-    format_A ++ format_string ◦ (constant close).
+  Definition format_with_term : FormatM A T :=
+    format_A ++ format_close ◦ (constant tt).
 
   Definition format_delimiter : FormatM A T :=
-    format_string ◦ (constant open) ++ format_with_term close.
+    format_open ◦ (constant tt) ++ format_with_term.
 
-  (* TODO: it is faster to take the size of [open]. *)
   Definition decode_delimiter
-             (decode_with_term :
-               string -> T -> CacheDecode -> option (A * T * CacheDecode))
-             (b : T) (cd : CacheDecode)
-    : option (A * T * CacheDecode) :=
-    `(s, b1, e1) <- decode_string (length open) b cd;
-    if String.eqb open s
-    then decode_with_term close b1 e1
-    else None.
+    (decode_with_term : DecodeM (A * T) T) :=
+    sequence_Decode decode_open (fun _ => decode_with_term).
 
-  Theorem delimiter_decode_correct
-          (decode_A_with_term
-            : string -> T -> CacheDecode -> option (A * T * CacheDecode))
-          (A_predicate : string -> A -> Prop)
-    : CorrectDecoder monoid (A_predicate close) (A_predicate close)
-                     eq (format_with_term close)
-                     (decode_A_with_term close)
-                     A_cache_inv
-                     (format_with_term close) ->
+  Variable decode_open_OK :
+    CorrectDecoder monoid (fun _ => True) (fun _ => True)
+        eq format_open
+        decode_open
+        A_cache_inv
+        format_open.
+
+  Variable decode_close_OK :
+    CorrectDecoder monoid (fun _ => True) (fun _ => True)
+        eq format_close
+        decode_close
+        A_cache_inv
+        format_close.
+
+  Variable decode_A_OK :
       CorrectDecoder monoid
-                     (A_predicate close)
-                     (A_predicate close)
-                     eq
-                     format_delimiter
-                     (decode_delimiter decode_A_with_term)
-                     A_cache_inv
-                     format_delimiter.
+        A_predicate
+        A_predicate
+        eq format_A
+        decode_A
+        A_cache_inv
+        format_A.
+
+  (* Just a variant of [format_sequence_correct]. Some parts can be generalized,
+  e.g., cache invariant. But this seems good enough for now. *)
+  Definition delimiter_decode_correct (decode_with_term : DecodeM (A * T) T)
+    : CorrectDecoder
+        monoid A_predicate A_predicate eq
+        format_with_term decode_with_term A_cache_inv
+        format_with_term ->
+      CorrectDecoder
+        monoid A_predicate A_predicate eq
+        format_delimiter (decode_delimiter decode_with_term) A_cache_inv
+        format_delimiter.
   Proof.
-    intros decode_A_OK.
-    eapply format_decode_correct_EquivDecoder_Proper; cycle 1.
-    - unfold format_delimiter.
-      eapply format_decode_correct_refineEquiv; unfold flip.
-
-      apply EquivFormat_UnderSequence.
-      eapply EquivFormat_trans.
-      apply EquivFormat_compose_id.
-      apply EquivFormat_sym.
-      apply sequence_mempty'.
-
-      eapply format_sequence_correct; cycle 1; intros; eauto.
-      eapply String_decode_correct; eauto. simpl; reflexivity.
-      eapply format_sequence_correct; intros; eauto. intuition eauto.
-
-      eapply CorrectDecoderEmpty. intuition eauto.
-
-      unfold IsProj.
-      instantiate (1:=(String.eqb _ _)).
-      match goal with
-      | |- context [String.eqb ?s ?s'] => destruct (String.eqb_spec s s')
-      end; simpl; solve [intuition eauto].
-
-      repeat instantiate (1:=constant True); split; eauto.
-
-    - intros t cd.
-      unfold sequence_Decode.
-      unfold decode_delimiter.
-      eapply DecodeBindOpt2_under_bind.
-      intros.
-      destruct String.eqb; subst; simpl;
-        destruct decode_A_with_term; destruct_conjs; reflexivity.
+    intros H.
+    eapply format_sequence_correct; intros; intuition eauto.
+    repeat instantiate (1:=fun _ => True); split; eauto.
+    destruct v1.
+    eapply weaken_source_pred; cycle -1.
+    eapply strengthen_view_pred; cycle -1.
+    eassumption.
+    all : repeat (hnf; intros; intuition).
   Qed.
 
-
-  Variable decode_A : T -> CacheDecode -> option (A * T * CacheDecode).
-  Variable A_predicate : A -> Prop.
-  Variable decode_A_OK : CorrectDecoder monoid A_predicate A_predicate
-                                        eq format_A
-                                        decode_A
-                                        A_cache_inv
-                                        format_A.
-
-  (* TODO: again, we should take the size of [close]. *)
-  Definition decode_with_term_simple (close : string)
-             (b : T) (cd : CacheDecode)
+  (* If [format_A] can be decoded individually. *)
+  Definition decode_with_term_simple (b : T) (cd : CacheDecode)
     : option (A * T * CacheDecode) :=
     `(a, b1, e1) <- decode_A b cd;
-    `(s, b2, e2) <- decode_string (length close) b1 e1;
-    if String.eqb close s
-    then Some (a, b2, e2)
-    else None.
+    `(_, b2, e2) <- decode_close b1 e1;
+    Some (a, b2, e2).
 
   Theorem decode_with_term_simple_correct
-    : CorrectDecoder monoid A_predicate A_predicate
-                     eq (format_with_term close)
-                     (decode_with_term_simple close)
-                     A_cache_inv
-                     (format_with_term close).
+    : CorrectDecoder
+        monoid A_predicate A_predicate eq
+        format_with_term
+        decode_with_term_simple
+        A_cache_inv
+        format_with_term.
   Proof.
+    unfold format_with_term, decode_with_term_simple.
     eapply format_decode_correct_EquivDecoder_Proper; cycle 1.
-    - unfold format_with_term.
-      eapply format_decode_correct_refineEquiv; unfold flip.
+    - eapply format_decode_correct_refineEquiv; unfold flip.
 
       apply EquivFormat_UnderSequence'.
       apply EquivFormat_compose_id.
       apply EquivFormat_sym.
       apply sequence_mempty'.
 
-      eapply format_sequence_correct; cycle 1; intros; eauto.
-      eapply format_sequence_correct; intros; eauto. intuition eauto.
-      eapply String_decode_correct; eauto. simpl; reflexivity.
-
+      eapply format_sequence_correct; cycle 1; intros; intuition eauto.
+      eapply format_sequence_correct; intros; intuition eauto.
       eapply CorrectDecoderEmpty. intuition eauto.
-
-      unfold IsProj.
-      instantiate (1:=(String.eqb _ _)).
-      match goal with
-      | |- context [String.eqb ?s ?s'] => destruct (String.eqb_spec s s')
-      end; simpl; solve [intuition eauto].
+      instantiate (1:=true).
+      unfold IsProj. simpl. intuition eauto. destruct v0; eauto.
 
       repeat instantiate (1:=constant True); split; eauto.
 
-    - intros t cd.
-      unfold sequence_Decode.
-      unfold decode_with_term_simple.
-      eapply DecodeBindOpt2_under_bind. intros.
-      eapply DecodeBindOpt2_under_bind. intros.
-      destruct String.eqb; subst; simpl; reflexivity.
+    - reflexivity.
   Qed.
 
   Definition decode_delimiter_simple :=
     decode_delimiter decode_with_term_simple.
 
   Corollary delimiter_decode_simple_correct
-    : CorrectDecoder monoid
-                     A_predicate
-                     A_predicate
-                     eq
-                     format_delimiter
-                     decode_delimiter_simple A_cache_inv
-                     format_delimiter.
+    : CorrectDecoder
+        monoid
+        A_predicate
+        A_predicate
+        eq
+        format_delimiter
+        decode_delimiter_simple A_cache_inv
+        format_delimiter.
   Proof.
-    eapply delimiter_decode_correct with (A_predicate := (fun _ => A_predicate)).
-    eapply decode_with_term_simple_correct.
+    intros.
+    eapply delimiter_decode_correct.
+    eapply decode_with_term_simple_correct; eauto.
   Qed.
 
 End Delimiter.
